Fad/Chapter3-Ex.lean
@@ -1,17 +1,15 @@
 import Fad.Chapter3
+import Fad.Chapter2
 
 namespace Chapter3Ex
 open Chapter3
 
 /-
-|  3.1 | Ana Luiza Nunes                        |
 | 3.12 | Anderson Gabriel Falcão dos Santos     |
-|  3.4 | Breno Russo Guedes de Souza Melo       |
-|  3.5 | Carlos Alberto de Souza Moreira Junior |
-|  3.2 | Gabriel Jacinto Pereira                |
+|  3.4 | Breno Russo Guedes de Souza Melo       | not
 | 3.10 | Henrique Coelho Beltrão                |
 |  3.9 | Jaime Willian Carneiro da Silva        |
-|  3.3 | Kauan Kevem Sousa Farias               |
+|  3.3 | Kauan Kevem Sousa Farias               | not
 | 3.14 | Leonardo Micheli Belo                  |
 |  3.8 | Luís Filipe Novaes de Souza            |
 | 3.15 | Nícolas Mateus Spaniol                 |
@@ -20,6 +18,72 @@ open Chapter3
 |  3.6 | Thiago Franke Melchiors                |
 | 3.13 | Wellington José Leite da Silva         |
 -/
+
+-- 3.1
+
+/-
+(['a', 'b', 'c'], ['d'])
+(['a'], ['d', 'c', 'b'])
+(['a', 'b'], ['d', 'c'])
+-/
+
+#eval toSL "abcd".toList
+#eval List.foldr consSL nilSL "abcd".toList
+#eval List.foldl (flip snocSL) nilSL "abcd".toList
+#eval consSL 'a' (snocSL 'd' (List.foldr consSL nilSL "bc".toList))
+
+
+-- 3.2
+
+-- I want prop?
+def nullSL {α : Type} : SymList α → Bool
+| (xs, ys) => xs.isEmpty ∧ ys.isEmpty
+
+def singleSL {α : Type} : SymList α → Prop
+| (xs, ys) => (xs.isEmpty ∧ single ys) ∨ (ys.isEmpty ∧ single xs)
+
+def lengthSL {α : Type} : SymList α → Nat
+| (xs, ys) => xs.length + ys.length
+
+
+-- 3.3
+
+def headSL? {α : Type} : SymList α → Option α
+ | ([],[])  => none    -- why not nilSL?
+ | ([], ys) => List.head? ys
+ | (xs, _)  => List.head? xs
+
+
+-- 3.4
+
+def initSL {α : Type} : SymList α → Option (SymList α)
+ | (xs, [])  => if xs.isEmpty then none else some nilSL
+ | (xs, [_]) =>
+   let (us, vs) := xs.splitAt (xs.length / 2)
+   some (us, vs.reverse)
+ | (xs, _ :: ys)  => some (xs, ys)
+
+
+-- 3.5
+
+def dropWhileSL (p : α → Bool) (sl : SymList α) : SymList α :=
+ let us := sl.1.dropWhile p
+ if us.isEmpty then toSL (sl.2.reverse.dropWhile p) else (us, sl.2)
+
+def dropWhileSL' (p : α → Bool) (sl : SymList α) : SymList α :=
+ match headSL? sl with
+ | none => nilSL
+ | some a =>
+   if p a then
+    match (tailSL sl) with
+    | none => nilSL
+    | some us => dropWhileSL p us
+   else sl
+
+-- #check decide (nullSL ([], []))  how to make it ?
+
+#eval [1,2,3,4].dropWhile (· < 3)
+#eval dropWhileSL (· < 3) (toSL [1,2,3,4]) |> fromSL
 
 
 end Chapter3Ex
